Suppose we have two number `a` and `b`, such that $a+b=0$. Then it is said that `a` and `b` are additive inverses of each other.

And for modulo `n` only whole number less than n are allowed, and the concept of additive inverses turn into
$$
\begin{align} \\
&\{a,b\in\mathbb{Z}\}\\
a+b&\equiv0\bmod{n}\\
\implies b&\equiv(0-a)\bmod{n} \\
\implies b&\equiv(-a)\bmod{n} \\
\implies b&=k*n-a&\forall k\in\mathbb{Z}
\end{align}
$$
and from this we have obtained the general expression for the additive inverse of `a`.